First heap lemma proven

theories/program_logic/weakestpre.v
@@ -1,10 +1,11 @@
+From iris.algebra Require Import auth gmap excl.
 From iris.proofmode Require Import base tactics classes.
 From iris.base_logic.lib Require Export fancy_updates.
 From shiris.program_logic Require Import state.
 Set Default Proof Using "Type".
 
 
-Definition state_wp `{invG Σ} {ST A} (SI: ST -> iProp Σ)
+Definition state_wp {Σ} {ST A} (SI: ST -> iProp Σ)
            (e: state ST A) (Φ: A -> iProp Σ): iProp Σ := ∀ σ,
   SI σ ==∗
   ∃ a σ', ⌜runState e σ = Some (a, σ') ⌝ ∗
@@ -12,7 +13,7 @@ Definition state_wp `{invG Σ} {ST A} (SI: ST -> iProp Σ)
           Φ a.
 
 Section state_wp.
-  Context `{invG Σ} {ST} (SI: ST -> iProp Σ).
+  Context  {Σ} {ST} (SI: ST -> iProp Σ).
   Implicit Types P Q R: iProp Σ.
 
   (*
@@ -41,42 +42,157 @@ Section state_wp.
   Qed.
 
 
-  Lemma fupd_wp {A} (e: state ST A) Φ : (|==> state_wp SI e Φ) ⊢ state_wp SI e Φ.
+  Lemma bupd_wp {A} (e: state ST A) Φ : (|==> state_wp SI e Φ) ⊢ state_wp SI e Φ.
   Proof.
     iIntros "Hwp" (σ) "HSi".
     iMod "Hwp" as "Hwp".
     iDestruct ("Hwp" $! σ with "HSi" ) as "$".
   Qed.
 
-  Lemma wp_fupd {A} (e: state ST A) Φ : state_wp SI e  (λ v, |==> Φ v) ⊢ state_wp SI e Φ.
+  Lemma wp_bupd {A} (e: state ST A) Φ : state_wp SI e  (λ v, |==> Φ v) ⊢ state_wp SI e Φ.
   Proof.
-    iIntros "Hwp" (σ) "HSi".
-    iMod ("Hwp" $! σ with "HSi") as (a σ') "(Hrun & HSi & HPhi)".
-    iMod "HPhi" as "HPhi".
-    eauto with iFrame.
+    iIntros "Hwp".
+    iApply (wp_strong_mono with "Hwp").
+    auto.
   Qed.
 
   Lemma wp_ret {A} (v: A) Φ: Φ v ⊢ state_wp SI (mret v) Φ.
   Proof.
-    iIntros "Hwp" (σ) "HSi".
-    iModIntro.
-    iExists v, σ.
+    iIntros "Hwp" (σ) "HSi !>".
     eauto with iFrame.
   Qed.
 
   Lemma wp_bind {A B} (e: state ST A) (f: A -> state ST B) Φ:
     state_wp SI e (λ v, state_wp SI (f v) Φ) ⊢ state_wp SI (e ≫= f) Φ.
   Proof.
-    iIntros "Hwp" (σ) "HSi".
-    iMod ("Hwp" $! (σ) with "HSi") as (x σ') "(Hrun & HSi' & Hwp')".
-    iMod ("Hwp'" $! (σ') with "HSi'") as (y σ'') "(Hrun' & HSi'' & Hpost)".
-    iModIntro.
-    iExists y, σ''.
-    simpl.
-    iDestruct "Hrun" as %->.
-    iDestruct "Hrun'" as %->.
+    iIntros "Hwp" (σ) "HSi /=".
+    iMod ("Hwp" $! (σ) with "HSi") as (x σ' ->) "(HSi' & Hwp')".
+    iMod ("Hwp'" $! (σ') with "HSi'") as (y σ'' ->) "(HSi'' & Hpost)".
     eauto with iFrame.
   Qed.
 
 
+  (*Derived rules *)
+  Lemma wp_mono {A} Φ Ψ (e: state ST A): (∀ v, Φ v ⊢ Ψ v) → state_wp SI e Φ ⊢ state_wp SI e Ψ.
+  Proof.
+     iIntros (HΦ) "H"; iApply (wp_strong_mono with "H"); auto.
+     iIntros (v) "?". by iApply HΦ.
+  Qed.
+
+  Lemma wp_value_fupd' {A} Φ (v: A) : (|==> Φ v) ⊢ state_wp SI (mret v) Φ.
+  Proof. by rewrite -wp_bupd -wp_ret. Qed.
+
 End state_wp.
+
+Definition heapR (A: ofeT): cmraT := authR (gmapUR nat (exclR A)).
+
+Section state_wp_gp.
+  Context `{! inG Σ (heapR natO)}.
+
+  About own.
+ (* Now come the rule that needs the points to connective in their weakest pre definition.
+     We therefore first define this in terms of the Authorative camera.
+   *)
+
+  Definition points_to (γ: gname) (n: nat) (v: nat): iProp Σ :=
+    own γ ( ◯ {[ n := Excl v ]}).
+
+  Definition lift_excl (σ: gmap nat nat): (gmap nat (excl nat)) := (Excl <$> σ).
+  Definition state_interp (γ: gname) (σ: gmap nat nat) := own γ (● (lift_excl σ)).
+
+
+  (*
+    I'm trying to prove that if I own an entire heap and I own a fragment of that heap then
+    Looking up the fragment in the heap will give me the value that corresponds to the fragment.
+
+    Robbert stated that the equality can be derived from the idea of validity.
+
+    The way to get from validity to equality is through singleton_included_exclusive.
+    Lets apply that first. It's hard to apply that since it is a pure statement, not one in a seperation logic context.
+    Instead let's try to build it's requirements, these are:
+    An x over which we have exclusive ownership, here: Excl v.
+    A map which is valid, we want: valid σ.
+    Then we have to show inclusion of the singleton in σ.
+
+    Step one: getting Valid of σ. Would be using own_valid on Hsi.
+    Step two: show inclusion of our singleton map in σ.
+              The lemma auth_both_valid gives us inclusion
+   *)
+  About auth_both_valid.
+  About singleton_included_exclusive.
+  Locate "=".
+  About Excl'.
+  About Excl.
+  SearchAbout equiv f_equal.
+  SearchAbout LeibnizEquiv.
+  SearchAbout fmap f_equal.
+  About leibniz_equiv_iff.
+  About f_equiv.
+
+  Lemma rewrite_lookups σ n v : lift_excl σ !! n ≡ Excl' v -> (σ !! n) = Some v.
+  Proof.
+    intros H.
+    rewrite (lookup_fmap Excl σ n) in H.
+    destruct (leibniz_equiv_iff (Excl <$> σ !! n) (Excl' v)).
+    apply H0 in H.
+    unfold fmap in H.
+    unfold option_fmap in H.
+    unfold option_map in H.
+    destruct (σ !! n) eqn: E.
+    - injection H. auto.
+    - discriminate H.
+  Qed.
+
+  Lemma bla γ σ n v: state_interp γ σ -∗ points_to γ n v -∗ ⌜σ !! n = Some v⌝.
+  Proof.
+    iIntros "Hsi Hpt".
+    unfold state_interp.
+    unfold points_to.
+    iDestruct (own_valid_2 with "Hsi Hpt") as "%".
+    pose (cmr := (gmapUR nat (exclR natO))).
+    pose (proj1 (@auth_both_valid cmr _ (lift_excl σ) ({[n := Excl v]}))).
+    destruct (a H) as [H1 H2].
+    iPureIntro.
+    pose (proj1 (singleton_included_exclusive (lift_excl σ) n (Excl v) _ H2) H1).
+    apply rewrite_lookups.
+    assumption.
+  Qed.
+
+   (* Todo state additional lemmas about the heap, alloc / store*)
+  (*usefull helper lemmas for combining owns *)
+  About own_valid.
+  About own_op.
+  About own_valid_2.
+  About own_update_2.
+  (*usefull helper lemmas for deriving equality from validity*)
+  SearchAbout auth valid.
+  SearchAbout excl.
+  About excl_valid.
+  Print excl_valid.
+  About auth_both_valid.
+  SearchAbout included gmap.
+  About singleton_included_exclusive.
+  About bi_iff.
+  About bi_and.
+  Locate "∧".
+  SearchAbout bi_iff.
+  SearchAbout bi_and.
+  SearchAbout fmap lookup.
+  About map_fmap_equiv_ext.
+  About lookup_fmap.
+  About map_fmap_ext.
+  About Excl'.
+
+  Lemma bla' γ σ n v w:
+    state_interp γ σ -∗ points_to γ n v ==∗ state_interp γ (<[n := w ]> σ) ∗ points_to γ n w.
+  Proof. Admitted.
+
+
+
+  Context (γ: gname).
+
+
+  Lemma wp_load n v (Ψ: nat -> iProp Σ) :
+    points_to γ n v -∗ (points_to γ n v -∗ Ψ v) -∗ state_wp (state_interp γ) (get _ n) Ψ.
+
+                       End. 
